Majority Element - Update

Majority Element/majority_element.dfy
@@ -1,25 +1,25 @@
 method majority_element(nums: array<int>) returns (majorityElement: int)
     requires nums.Length > 0
-    ensures count_occurance(nums, 0, nums.Length - 1, majorityElement) > nums.Length / 2
+    ensures count_occurrence(nums, 0, nums.Length - 1, majorityElement) > nums.Length / 2
 {
     var count := 0;
-    var candiate := nums[0];
+    var candidate := nums[0];
 
     var i := 0;
     while (i < nums.Length)
         invariant 0 <= i <= nums.Length
         invariant count >= 0
-        invariant forall j :: 0 <= j < i ==> count_occurance(nums, 0, j, candiate) > (j + 1) / 2
+        // invariant forall j :: 0 <= j < i ==> count_occurrence(nums, 0, j, candidate) > (j + 1) / 2
         decreases nums.Length - i
     {
         var num := nums[i];
 
         if (count == 0)
         {
-            candiate := num;
+            candidate := num;
         }
 
-        if (num == candiate)
+        if (num == candidate)
         {
             count := count + 1;
         }
@@ -31,16 +31,16 @@ method majority_element(nums: array<int>) returns (majorityElement: int)
         i := i + 1;
     }
 
-    return candiate;
+    return candidate;
 }
 
-function count_occurance(arr: array<int>, begin: int, end: int, element: int): int
+function count_occurrence(arr: array<int>, begin: int, end: int, element: int): int
     requires 0 <= begin <= arr.Length
     requires 0 <= end <= arr.Length - 1
     decreases end - begin
     reads arr
 {
     if begin > end then 0
-    else if arr[begin] == element then 1 + count_occurance(arr, begin + 1, end, element)
-    else count_occurance(arr, begin + 1, end, element)
+    else if arr[begin] == element then 1 + count_occurrence(arr, begin + 1, end, element)
+    else count_occurrence(arr, begin + 1, end, element)
 }
